fstar-helpers/fstar-bitvec/BitVec.Utils.fst
@@ -1,0 +1,21 @@
+module BitVec.Utils
+
+open Core
+open FStar.FunctionalExtensionality
+open BitVec.Equality
+open Rust_primitives.BitVectors
+
+let mk_bv #len (f: (i:nat{i < len}) -> bit) = on (i:nat {i < len}) f
+
+let mk_list_32 #a (x0 x1 x2 x3 x4 x5 x6 x7 x8 x9 x10 x11 x12 x13 x14 x15 x16 x17 x18 x19 x20 x21 x22 x23 x24 x25 x26 x27 x28 x29 x30 x31: a)
+  : (l:list a {List.Tot.length l == 32})
+  = let l = [x0;x1;x2;x3;x4;x5;x6;x7;x8;x9;x10;x11;x12;x13;x14;x15;x16;x17;x18;x19;x20;x21;x22;x23;x24;x25;x26;x27;x28;x29;x30;x31] in
+    assert_norm (List.Tot.length l == 32);
+    l
+
+let mk_list_8 #a (x0 x1 x2 x3 x4 x5 x6 x7: a)
+  : (l:list a {List.Tot.length l == 8})
+  = let l = [x0;x1;x2;x3;x4;x5;x6;x7] in
+    assert_norm (List.Tot.length l == 8);
+    l
+
